chore

Auto/Embedding/LamThm.lean
@@ -2,6 +2,19 @@ import Auto.Embedding.LamBase
 
 namespace Auto.Embedding.Lam
 
+structure LamThmJudge where
+  lctx  : List LamSort
+  rterm : LamTerm
+  rty   : LamSort
+
+def LamThmWF (lval : LamValuation) (ltj : LamThmJudge) :=
+  ∀ (lctx' : Nat → LamSort), LamWF lval.ilVal.toLamTyVal ⟨pushLCtxs lctx' ltj.lctx, ltj.rterm, ltj.rty⟩
+
+def LamThmValid (lval : LamValuation) (lctx : List LamSort) (t : LamTerm) :=
+  ∀ (lctx' : Nat → LamSort) (lctxTerm : ∀ n, (pushLCtxs lctx' lctx n).interp lval.ilVal.tyVal),
+    ∃ (wf : LamWF lval.ilVal.toLamTyVal ⟨pushLCtxs lctx' lctx, t, .base .prop⟩),
+      GLift.down (LamWF.interp lval (pushLCtxs lctx' lctx) lctxTerm wf)
+
 def Eq.symm.WF (wf : LamWF ltv ⟨lctx, .app (.app (.base (.eq n)) a) b, .base .prop⟩) :
   LamWF ltv ⟨lctx, .app (.app (.base (.eq n)) b) a, .base .prop⟩ :=
   match wf with
@@ -13,7 +26,7 @@ def Eq.symm.WF (wf : LamWF ltv ⟨lctx, .app (.app (.base (.eq n)) a) b, .base .
         match HB with
         | .ofEq n => .ofApp _ (.ofApp _ (.ofBase (.ofEq n)) wfB) wfA
 
-theorem Eq.symm (lval : LamValuation)
+theorem Eq.symmAux (lval : LamValuation)
   {lctxTy : Nat → LamSort} {lctxTerm : ∀ n, (lctxTy n).interp lval.ilVal.tyVal}
   (wf : LamWF lval.ilVal.toLamTyVal ⟨lctxTy, .app (.app (.base (.eq n)) a) b, .base .prop⟩)
   (H : GLift.down (LamWF.interp lval lctxTy lctxTerm wf)) :
@@ -28,6 +41,16 @@ theorem Eq.symm (lval : LamValuation)
         have H' := EqLift.down _ _ _ H
         apply EqLift.up
         exact (_root_.Eq.symm H')
+
+theorem Eq.symm (lval : LamValuation) (lctx : List LamSort)
+  (H : LamThmValid lval lctx (.app (.app (.base (.eq n)) a) b)) :
+  LamThmValid lval lctx (.app (.app (.base (.eq n)) b) a) := by
+  unfold LamThmValid; unfold LamThmValid at H
+  intros lctx' lctxTerm
+  cases (H lctx' lctxTerm)
+  case intro wf H =>
+    exists Eq.symm.WF wf
+    apply Eq.symmAux _ _ H
 
 def Eq.trans.WF
   (wf₁ : LamWF ltv ⟨lctx, .app (.app (.base (.eq m)) a) b, .base .prop⟩)
@@ -53,7 +76,7 @@ def Eq.trans.WF
                     (LamWF.unique ltv wfB₁ wfB₂).left
                   .ofApp _ (.ofApp _ (.ofBase (.ofEq n)) (heq ▸ wfA)) wfC
 
-theorem Eq.trans (lval : LamValuation)
+theorem Eq.transAux (lval : LamValuation)
   {lctxTy : Nat → LamSort} {lctxTerm : ∀ n, (lctxTy n).interp lval.ilVal.tyVal}
   (wf₁ : LamWF lval.ilVal.toLamTyVal ⟨lctxTy, .app (.app (.base (.eq m)) a) b, .base .prop⟩)
   (H₁ : GLift.down (LamWF.interp lval lctxTy lctxTerm wf₁))
@@ -88,6 +111,19 @@ theorem Eq.trans (lval : LamValuation)
                   case a.h.h₂ =>
                     rw [H₁']; rw [← H₂']; apply LamWF.interp.heq <;> rfl
 
+theorem Eq.trans (lval : LamValuation) (lctx : List LamSort)
+  (H₁ : LamThmValid lval lctx (.app (.app (.base (.eq n)) a) b))
+  (H₂ : LamThmValid lval lctx (.app (.app (.base (.eq n)) b) c)) :
+  LamThmValid lval lctx (.app (.app (.base (.eq n)) a) c) := by
+  unfold LamThmValid; unfold LamThmValid at H₁ H₂
+  intros lctx' lctxTerm
+  cases (H₁ lctx' lctxTerm)
+  case intro wf₁ H₁ =>
+    cases (H₂ lctx' lctxTerm)
+    case intro wf₂ H₂ =>
+      exists Eq.trans.WF wf₁ wf₂
+      apply Eq.transAux _ _ H₁ _ H₂
+
 def Eq.subst.WF
   (wfEq : LamWF ltv ⟨lctx, .app (.app (.base (.eq n)) a) b, .base .prop⟩)
   (wfP : LamWF ltv ⟨lctx, .app p a, .base .prop⟩) :
@@ -106,7 +142,7 @@ def Eq.subst.WF
               (LamWF.unique ltv wfA wfA').left
             .ofApp _ wfP (heq ▸ wfB)
 
-theorem Eq.subst (lval : LamValuation)
+theorem Eq.substAux (lval : LamValuation)
   {lctxTy : Nat → LamSort} {lctxTerm : ∀ n, (lctxTy n).interp lval.ilVal.tyVal}
   (wfEq : LamWF lval.ilVal.toLamTyVal ⟨lctxTy, .app (.app (.base (.eq m)) a) b, .base .prop⟩)
   (hEq : GLift.down (LamWF.interp lval lctxTy lctxTerm wfEq))
@@ -133,6 +169,19 @@ theorem Eq.subst (lval : LamValuation)
             case h.h.h.h₂ =>
               rw [hEq']; apply LamWF.interp.heq <;> rfl
 
+theorem Eq.subst (lval : LamValuation) (lctx : List LamSort)
+  (hEq : LamThmValid lval lctx (.app (.app (.base (.eq n)) a) b))
+  (hP : LamThmValid lval lctx (.app p a)) :
+  LamThmValid lval lctx (.app p b) := by
+  unfold LamThmValid; unfold LamThmValid at hEq hP
+  intros lctx' lctxTerm
+  cases (hEq lctx' lctxTerm)
+  case intro wfEq hEq =>
+    cases (hP lctx' lctxTerm)
+    case intro wfP hP =>
+      exists Eq.subst.WF wfEq wfP
+      apply Eq.substAux _ _ hEq _ hP
+
 def Eq.congr.WF
   (wfEq : LamWF ltv ⟨lctx, .app (.app (.base (.eq n)) a) b, .base .prop⟩)
   (wfT : LamWF ltv ⟨lctx, .app f a, s⟩)
@@ -152,10 +201,10 @@ def Eq.congr.WF
             (.ofApp _ (.ofBase (.ofEq _))
             (.ofApp _ wfF (heq ▸ wfA))) (.ofApp _ wfF (heq ▸ wfB))
 
-def Eq.congr (lval : LamValuation)
+theorem Eq.congrAux (lval : LamValuation)
   {lctxTy : Nat → LamSort} {lctxTerm : ∀ n, (lctxTy n).interp lval.ilVal.tyVal}
   (wfEq : LamWF lval.ilVal.toLamTyVal ⟨lctxTy, .app (.app (.base (.eq m)) a) b, .base .prop⟩)
-  (heq : GLift.down (LamWF.interp lval lctxTy lctxTerm wfEq))
+  (hEq : GLift.down (LamWF.interp lval lctxTy lctxTerm wfEq))
   (wfT : LamWF lval.ilVal.toLamTyVal ⟨lctxTy, .app f a, s⟩)
   (wfEq' : LamWF lval.ilVal.toLamTyVal ⟨lctxTy, .base (.eq m), .func s (.func s (.base .prop))⟩) :
   GLift.down (LamWF.interp lval lctxTy lctxTerm (Eq.congr.WF wfEq wfT wfEq')) :=
@@ -168,12 +217,28 @@ def Eq.congr (lval : LamValuation)
         match wfT with
         | .ofApp aTy' wfF wfA' => by
           dsimp [trans.WF, LamWF.interp, LamBaseWF.interp];
-          dsimp [trans.WF, LamWF.interp, LamBaseWF.interp] at heq;
+          dsimp [trans.WF, LamWF.interp, LamBaseWF.interp] at hEq;
           apply EqLift.up;
-          have heq' := EqLift.down _ _ _ heq
+          have heq' := EqLift.down _ _ _ hEq
           apply congrArg; apply eq_of_heq
           apply HEq.trans (b:=LamWF.interp lval lctxTy lctxTerm wfA)
           case a.h.h.h₁ => apply LamWF.interp.heq <;> rfl
           case a.h.h.h₂ => rw [heq']; apply LamWF.interp.heq <;> rfl
+
+theorem Eq.congr (lval : LamValuation) (lctx : List LamSort)
+  (hEq : LamThmValid lval lctx (.app (.app (.base (.eq m)) a) b))
+  (wfT : LamThmWF lval ⟨lctx, .app f a, s⟩)
+  (wfEq' : LamThmWF lval ⟨lctx, .base (.eq m), .func s (.func s (.base .prop))⟩) :
+  LamThmValid lval lctx (.app (.app (.base (.eq m)) (.app f a)) (.app f b)) := by
+  unfold LamThmValid; unfold LamThmValid at hEq; unfold LamThmWF at wfT wfEq'
+  intros lctx' lctxTerm
+  cases (hEq lctx' lctxTerm)
+  case intro wfEq hEq =>
+    let wfT := wfT lctx'
+    let wfEq' := wfEq' lctx'
+    exists (Eq.congr.WF wfEq wfT wfEq')
+    apply Eq.congrAux _ wfEq hEq wfT wfEq'
+
+attribute [irreducible] LamThmWF LamThmValid
 
 end Auto.Embedding.Lam
