Auto/Examples/FirstOrder.lean
@@ -12,6 +12,7 @@ open Classical
 variable (α : Type) (p q : α → Prop)
 variable (r : Prop)
 
+set_option smt.solver.name "cvc5"
 example : (∃ x : α, r) → r := by
   try auto;
   sorry
