Auto/Lib/BinNat.lean
@@ -1,0 +1,119 @@
+inductive Pos where
+  | xH : Pos
+  | xO : Pos → Pos
+  | xI : Pos → Pos
+deriving Inhabited
+
+abbrev Pos.one := xH
+
+inductive Bin where
+  | zero : Bin
+  | pos : Pos → Bin
+
+abbrev Bin.one := pos .xH
+
+def Pos.beq : (p q : Pos) → Bool
+| xH,    xH    => true
+| xO p', xO q' => p'.beq q'
+| xI p', xI q' => p'.beq q'
+| _,     _     => false
+
+theorem Pos.beq_refl (p : Pos) : p.beq p = true := by
+  induction p
+  case xH => rfl
+  case xO p' IH => simp [beq, IH]
+  case xI p' IH => simp [beq, IH]
+
+theorem Pos.beq_eq : (p q : Pos) → p.beq q = true → p = q
+| xH,    xH    => fun _ => rfl
+| xH,    xO  _ => fun H => by cases H
+| xH,    xI _  => fun H => by cases H
+| xO _,  xH    => fun H => by cases H
+| xO p', xO q' => fun H => by simp [beq, Pos.beq_eq p' q' H]
+| xO p', xI q' => fun H => by cases H
+| xI _,  xH    => fun H => by cases H
+| xI _,  xO _  => fun H => by cases H
+| xI p', xI q' => fun H => by simp [beq, Pos.beq_eq p' q' H]
+
+instance : BEq Pos where
+  beq := Pos.beq
+
+private partial def Pos.ofNatAux (n : Nat) :=
+  match n with
+  | 0 => xH
+  | 1 => xH
+  | _ =>
+    match n % 2 with
+    | 0 => .xO (Pos.ofNatAux (n / 2))
+    | _ => .xI (Pos.ofNatAux (n / 2))
+
+def Pos.succ (p : Pos) : Pos :=
+  match p with
+  | xH     => .xO .xH
+  | .xO p' => .xI p'
+  | .xI p' => .xO (Pos.succ p')
+
+def Pos.predXO : Pos → Pos
+| xH   => xH
+| xO p => xI (predXO p)
+| xI p => xI (xO p)
+
+def Pos.pred (p : Pos) : Pos :=
+  match p with
+  | xH      => .xH
+  | xO p'  => p'.predXO
+  | xI p'  => .xO p'
+
+def Bin.ofPredPos : (p : Pos) → Bin
+| .xH    => zero
+| .xO p' => pos (.predXO p')
+| .xI p' => pos (.xO p')
+
+theorem Pos.succ_neq (p : Pos) : p ≠ Pos.succ p := by
+  cases p <;> intro h <;> contradiction
+
+theorem Pos.pred_neq (p : Pos) : p ≠ .xH → p ≠ Pos.pred p := by
+  cases p <;> intro h₁ h₂ <;> try contradiction
+  case xO p' => cases p' <;> try contradiction
+
+theorem Pos.predXO_spec (p : Pos) : p.predXO = (xO p).pred := by
+  cases p <;> rfl
+
+theorem Pos.succ_predXO (p : Pos) : succ (predXO p) = xO p := by
+  induction p <;> try rfl
+  case xO a IH => simp [predXO, succ, IH]
+
+theorem Pos.predXO_succ (p : Pos) : predXO (succ p) = xI p := by
+  induction p <;> try rfl
+  case xI a IH => simp [predXO, succ, IH]
+
+theorem Pos.double_succ (p : Pos) : xO (succ p) = succ (succ (xO p)) := by
+  cases p <;> rfl
+
+theorem Pos.predXO_neq_xO (p : Pos) : predXO p ≠ xO p := by
+  cases p <;> intro h <;> contradiction
+
+theorem succ_not_1 (p : Pos) : Pos.succ p ≠ .one := by
+  cases p <;> intro h <;> try contradiction
+
+theorem Pos.pred_succ_eq (p : Pos) : Pos.pred (.succ p) = p := by
+  cases p <;> try rfl
+  case xI p' => apply predXO_succ
+
+theorem Pos.succ_pred_xO (p : Pos) : succ (pred (xO p)) = xO p := by
+  induction p <;> try rfl
+  case xO p' IH =>
+    dsimp [succ, pred]; dsimp [succ, pred] at IH; rw [IH]
+
+theorem Pos.succ_pred_xI (p : Pos) : succ (pred (xI p)) = xI p := by
+  cases p <;> rfl
+
+theorem Pos.neq_XH_succ_pred_eq (p : Pos) : p ≠ .xH → Pos.succ (Pos.pred p) = p := by
+  cases p <;> intro h
+  case xH => contradiction
+  case xO _ => apply Pos.succ_pred_xO
+  case xI _ => apply Pos.succ_pred_xI
+
+theorem Pos.succ_inj (p q : Pos) : Pos.succ p = Pos.succ q → p = q := fun H =>
+  Pos.pred_succ_eq p ▸ Pos.pred_succ_eq q ▸ (congrArg _ H : pred (succ p) = pred (succ q))
+
