Auto/Lib/BinTree.lean
@@ -1,0 +1,31 @@
+import Auto.Lib.BinNat
+
+inductive BinTree (α : Sort _) where
+  | leaf : BinTree α
+  | node : BinTree α → α → BinTree α → BinTree α
+
+def BinTree.val (bt : BinTree α) (default : α) :=
+  match bt with
+  | .leaf => default
+  | .node _ x _ => x
+
+def BinTree.left (bt : BinTree α) :=
+  match bt with
+  | .leaf => BinTree.leaf
+  | .node l _ _ => l
+
+def BinTree.right (bt : BinTree α) :=
+  match bt with
+  | .leaf => BinTree.leaf
+  | .node _ _ r => r
+
+def BinTree.get (bt : BinTree α) (default : α) (bs : Pos) :=
+  match bs with
+  | .xH => bt.val default
+  | .xO bs' => BinTree.get bt.left default bs'
+  | .xI bs' => BinTree.get bt.right default bs'
+    
+structure QList (α : Sort _) where
+  data : BinTree α
+  size : Nat
+  default : α
