Auto/Solver/SMT.lean
@@ -68,7 +68,7 @@ def createSolver (name : SolverName) : MetaM SolverProc := do
   match name with
   | .z3   => createAux "z3" #["-in", "-smt2"]
   | .cvc4 => throwError "cvc4 is not supported"
-  | .cvc5 => throwError "cvc5 is not supported"
+  | .cvc5 => createAux "cvc5" #[]
 where
   createAux (path : String) (args : Array String) : MetaM SolverProc :=
     IO.Process.spawn {stdin := .piped, stdout := .piped, stderr := .piped,
