Test/Reduction.lean
@@ -6,3 +6,17 @@ set_option maxRecDepth 50000 in
 
 set_option maxRecDepth 50000 in
 #lazyReduce (List.range 10000).length
+
+#check 2
+
+#check Classical.propDecidable
+#check fun (α : Type) (i : LE α) (x y : α) => x <= y
+#check trans
+#check LE.le
+
+def casting (f g : Nat → Type) (x : ∀ n, f n) (H : ∀ n, f n = g n) : (∀ n, g n) :=
+  let heq : f = g := funext (fun n => H n);
+  heq ▸ x
+
+#eval casting (fun n => Nat) (fun n => match n with | 0 => Nat | _ => Nat) (fun n => n)
+  (fun n => by cases n <;> rfl) 21
